@prefix bsm: <http://w3id.org/besocial/ns/model#> .
@prefix owl: <http://www.w3.org/2002/07/owl#> .
@prefix rdf: <http://www.w3.org/1999/02/22-rdf-syntax-ns#> .
@prefix rdfs: <http://www.w3.org/2000/01/rdf-schema#> .
@prefix foaf: <http://xmlns.com/foaf/0.1/> .
@prefix cc: <http://creativecommons.org/ns#> .
@prefix dc: <http://purl.org/dc/terms/> .
@prefix xsd: <http://www.w3.org/2001/XMLSchema#> .
@prefix prov: <http://www.w3.org/ns/prov#> .
@prefix qb: <http://purl.org/linked-data/cube#> .
@prefix vann: <http://purl.org/vocab/vann/> .
@prefix edm: <http://www.europeana.eu/schemas/edm/> .
@prefix premis: <http://www.loc.gov/premis/rdf/v3/> .

<https://w3id.org/besocial/ns/model#> rdf:type owl:Ontology ;
                                       vann:preferredNamespacePrefix "bsm" ;
                                       vann:preferredNamespaceUri "https://w3id.org/besocial/ns/model#" ;
                                       rdfs:label "BESOCIAL vocabulary"@en ;
                                       dc:title "BESOCIAL vocabulary"@en ;
                                       dc:description "The BESOCIAL vocabulary used to describe social media archives"@en ;
                                       rdfs:comment """-Version 1.0.0: Initial version introduces needed classes."""@en ;
                                       owl:versionIRI   <https://w3id.org/besocial/ns/model/v1.0.0#> ;
                                       owl:versionInfo "1.0.0" ;
                                       owl:priorVersion <https://w3id.org/besocial/ns/model#> ;
                                       rdfs:seeAlso <https://w3id.org/besocial> ;
                                       dc:modified "2021-07-30"^^xsd:date ;
                                       dc:issued "2021-07-30"^^xsd:date ;
                                       dc:created "2021-07-30"^^xsd:date ;
                                       dc:rights "Copyright © Ghent University – imec – IDLab"@en ;
                                       cc:license <https://creativecommons.org/licenses/by/4.0/> ;
                                       foaf:primaryTopic <https://w3id.org/besocial> ;
                                       dc:creator <https://sven-lieber.org/profile#me> .

#
# Classes
#
bsm:SocialMediaCollection a rdfs:Class ;
  rdfs:label "SocialMediaCollection"@en ;
  rdfs:comment "A social media collection which is a premis:IntellectualEntity, edm:ProvidedCHO and prov:Entity"@en ;
  rdfs:subClassOf edm:ProvidedCHO, premis:IntellectualEntity, prov:Entity .

bsm:SocialMediaCollectionRepresentation a rdfs:Class ;
  rdfs:label "SocialMediaCollectionRepresentation"@en ;
  rdfs:comment "A social media collection representation which is a premis:Representation, edm:WebResource and prov:Entity, for example a representation in JSON."@en ;
  rdfs:subClassOf edm:WebResource, premis:Representation, prov:Entity .

bsm:SocialMediaCollectionRepresentationVersion a rdfs:Class ;
  rdfs:label "SocialMediaCollectionRepresentationVersion"@en ;
  rdfs:comment "A specific version of a social media collection representation which is a premis:Representation, edm:WebResource and prov:Entity, for example a representation in JSON."@en ;
  rdfs:subClassOf edm:WebResource, premis:Representation, prov:Entity .

bsm:SocialMediaPostsObservation a rdfs:Class ;
  rdfs:label "SocialMediaPostsObservation"@en ;
  rdfs:comment "A data cube observation regarding a number of social media posts."@en ;
  rdfs:subClassOf qb:Observation . 


#
# Named individuals
#
bsm:collectionDimension a qb:DimensionProperty, rdf:Property ;
  rdfs:label "collectionDimension"@en ;
  rdfs:comment "The collection to which this observation relates to."@en .

bsm:collectionRepresentationDimension a qb:DimensionProperty, rdf:Property ;
  rdfs:label "collectionRepresentationDimension"@en ;
  rdfs:comment "The collection representation this observation relates to, e.g. a JSON representation."@en .

bsm:collectionRepresentationVersionDimension a qb:DimensionProperty, rdf:Property ;
  rdfs:label "collectionRepresentationVersionDimension"@en ;
  rdfs:comment "The collection representation version this observation relates to, e.g. the version 2020100416 of a JSON representation."@en .

bsm:monthDimension a qb:DimensionProperty, rdf:Property ;
  rdfs:label "monthDimension"@en ;
  rdfs:comment "The month this observation relates to."@en .

bsm:yearDimension a qb:DimensionProperty, rdf:Property ;
  rdfs:label "yearDimension"@en ;
  rdfs:comment "The year this observation relates to."@en .


bsm:numberPosts a qb:MeasureProperty, rdf:Property ;
  rdfs:label "numberPosts"@en ;
  rdfs:comment "Number of social media posts. For example 55 social media posts such as 55 tweets."@en .
